coq/lib/Utils/Util/ListUtil.v
@@ -1,5 +1,5 @@
 Require Import Coq.Strings.String.
-From Poulet4 Require Export Utils.Util.FunUtil Utils.Util.StringUtil Monads.Result.
+From Poulet4 Require Export Utils.Util.FunUtil Utils.Util.StringUtil Monads.Result Monads.Option.
 From Coq Require Export Lists.List micromega.Lia.
 Export ListNotations.
 Require VST.zlist.sublist.
@@ -295,6 +295,91 @@ Section FoldRighti.
     snd (List.fold_right (fun a '(i, b) => (i + 1, f i a b )) (O, init) xs).
 End FoldRighti.
 
+Fixpoint partitions {A : Type} (l : list A) : list (list A * list A) :=
+  match l with
+  | [] => [([], [])]
+  | h :: t => ([], l) :: List.map (fun '(l1, l2) => (h :: l1, l2)) (partitions t)
+  end.
+
+Lemma partitions_sound :
+  forall (A : Type) (l l1 l2 : list A),
+    In (l1, l2) (partitions l) -> l1 ++ l2 = l.
+Proof.
+  induction l; cbn; intros l1 l2 [? | ?].
+  - inv H. reflexivity.
+  - contradiction.
+  - inv H. reflexivity.
+  - rewrite in_map_iff in H. inv H.
+    destruct x. inv H0. inv H.
+    apply IHl in H1. subst. reflexivity.
+Qed.
+
+Fixpoint find_map {A B : Type} (f : A -> option B) (l : list A) : option B :=
+  match l with
+  | [] => None
+  | h :: t =>
+    match f h with
+    | Some _ as v => v
+    | None => find_map f t
+    end
+  end.
+
+Lemma find_map_sound :
+  forall (A B : Type) (f : A -> option B) (l : list A) (v : B),
+    find_map f l = Some v -> exists x, In x l /\ f x = Some v.
+Proof.
+  induction l.
+  - discriminate.
+  - cbn. intros. destruct (f a) eqn:E.
+    + inv H. exists a. auto.
+    + apply IHl in H. inv H. inv H0. exists x. auto.
+Qed.
+
+Fixpoint split_at {A : Type} (n : nat) (l : list A) :=
+  match n with
+  | O => Some ([], l)
+  | S k =>
+    match l with
+    | [] => None
+    | h :: t =>
+      let^ '(l1, l2) := split_at k t in
+      (h :: l1, l2)
+    end
+  end.
+
+Lemma split_at_partition :
+  forall (A : Type) (n : nat) (l l1 l2 : list A),
+    split_at n l = Some (l1, l2) -> l1 ++ l2 = l.
+Proof.
+  induction n.
+  - cbn. intros. inv H. reflexivity.
+  - cbn. intros. destruct l; try discriminate.
+    unfold option_bind in *.
+    destruct (split_at n l) eqn:E; try discriminate.
+    destruct p. apply IHn in E. inv H. reflexivity.
+Qed.
+
+Lemma split_at_length_l1 :
+  forall (A : Type) (n : nat) (l l1 l2 : list A),
+    split_at n l = Some (l1, l2) -> List.length l1 = n.
+Proof.
+  induction n.
+  - cbn. intros. inv H. reflexivity.
+  - cbn. unfold option_bind. intros.
+    destruct l; try discriminate.
+    destruct (split_at n l) eqn:E; try discriminate.
+    destruct p. inv H. cbn. eauto.
+Qed.
+
+Lemma split_at_length_l2 :
+  forall (A : Type) (n : nat) (l l1 l2 : list A),
+    split_at n l = Some (l1, l2) -> List.length l2 = List.length l - n.
+Proof.
+  intros. apply split_at_length_l1 in H as ?.
+  apply split_at_partition in H as ?.
+  assert (List.length (l1 ++ l2) = List.length l1 + List.length l2) by apply app_length.
+  rewrite H1 in H2. lia.
+Qed.
 
 Section FoldLefti.
   Context {A B : Type}.
